src/Init/Data/Range/New/NatLemmas.lean
@@ -1,0 +1,15 @@
+module
+
+prelude
+import Init.Data.Range.New.Nat
+import Init.Data.Range.New.Lemmas
+
+namespace Std.PRange
+
+-- -- idea: show that toList = range'
+-- @[simp] theorem forIn'_eq_forIn'_range' [Monad m] (r : PRange ⟨.closed, .open⟩ Nat)
+--     (init : β) (f : (a : Nat) → a ∈ r → β → m (ForInStep β)) :
+--     forIn' r init f =
+--       forIn' (List.range' r.lower r.size 1) init (fun a h => f a (mem_of_mem_range' h)) := by
+
+end Std.PRange
